Infinite sequences, traces, omega languages

theories/example.v
@@ -1,6 +1,33 @@
-Require Import Automatik.pset.
-Require Import Automatik.operators.
+Require Import Automatik.lib.pset.
+Require Import Automatik.lib.sequence.
+Require Import Automatik.lib.operators.
+Require Import List.
+Import ListNotations.
 
 Definition P : pset nat := fun x => x = 1.
 Definition Q : pset nat := fun x => x = 2.
 Definition R : pset nat := P ∩ Q.
+
+Definition s1 : sequence.t nat := fun x => x + 1.
+Definition s2 : sequence.t nat := fun x => x + 2.
+Definition s3 := s1⟨1+⟩.
+
+Goal s2 ≡ s3.
+Proof.
+  unfold s2, s3. unfold s1.
+  intros i. cbn.
+  Require Import Lia.
+  lia.
+Qed.
+
+Goal s1⟨1…3⟩ = [2; 3 ; 4].
+Proof.
+  reflexivity.
+Qed.
+
+Definition s4 := sequence.repeat 0 [1; 2; 3].
+
+Goal s4⟨0…5⟩ = [1; 2; 3; 1; 2; 3].
+Proof.
+  reflexivity.
+Qed.
