theories/model.v
@@ -1,12 +1,15 @@
-(** Coq Model of Graphs/Automaton *)
+(** * Coq Model of Graphs/Automaton *)
 
-Require Import Automatik.operators Automatik.pset.
-Require Import List.
+Require Import Automatik.lib.operators Automatik.lib.pset Automatik.lib.sequence.
+Require Import List Relations.Relation_Operators.
 Import ListNotations.
 
 Section Model.
 
+(** Type of states *)
 Variable S : Type.
+
+(** Type of labels (alphabet) *)
 Variable A : Type.
 
 
@@ -33,12 +36,15 @@ Definition step (m : t) (x y : S) :=
   exists a, lstep m x a y.
 Instance step_op : StepOp t S := step.
 
+Definition steps (m : t) :=
+  clos_refl_trans_1n _ (step m).
+Instance steps_op : StepsOp t S := steps.
 
 (** ** Properties of Automaton *)
 
 
 (** What it means to be deterministic *)
-Definition Determinist (m : t) : Prop :=
+Definition Deterministic (m : t) : Prop :=
   forall s,
     m_relation m s = [] \/
     exists s', m_relation m s = [s'].
@@ -46,6 +52,10 @@ Definition Determinist (m : t) : Prop :=
 (** What it means to be complete *)
 Definition Complete (m : t) : Prop :=
   forall s a, exists s',
+    m $ s -[a]-> s'.
+
+Definition NonBlocking (m : t) : Prop :=
+  forall s, exists a s',
     m $ s -[a]-> s'.
 
 
@@ -73,8 +83,12 @@ Inductive FinPath (m : t) : S -> fin_path -> S -> Prop :=
 Instance FinPath_lsteps_op : LstepsOp t S (list (A * S)) := FinPath.
 
 (** The set of valid pathes of a graph. *)
-Definition Pathes (m : t) (s : S) : pset fin_path :=
+Definition FinPathes (m : t) (s : S) : pset fin_path :=
   fun p => exists s', m $ s -[p]->* s'.
+
+(** The set of intial pathes of a graph. *)
+Definition iFinPathes (m : t) : pset fin_path :=
+  fun p => exists s0, In s0 (m_initial m) /\ FinPathes m s0 p.
 
 (** What it means to be a valid finite trace in
     a graph.
@@ -89,11 +103,15 @@ Inductive FinTrace (m : t) : S -> fin_trace -> S -> Prop :=
 Instance FinTrace_lsteps_op : LstepsOp t S (list S) := FinTrace.
 
 (** The set of valid traces of a graph. *)
-Definition Traces (m : t) (s : S) : pset fin_trace :=
+Definition FinTraces (m : t) (s : S) : pset fin_trace :=
   fun t => exists s', m $ s -[t]->* s'.
 
-(** What it means to be a finite word starting in 
-    an automata.
+(** The set of initial traces of a graph. *)
+Definition iFinTraces (m : t) : pset fin_trace :=
+  fun t => exists s0, In s0 (m_initial m) /\ FinTraces m s0 t.
+
+(** What it means to be a finite word starting from
+    a given state in an automata.
 *)
 Inductive FinWord (m : t) : S -> fin_word -> Prop :=
   | fin_word_empty_ x : FinWord m x []
@@ -104,7 +122,7 @@ Inductive FinWord (m : t) : S -> fin_word -> Prop :=
 
 (** The set of valid (finite) words starting in a given state
     of an automata. *)
-Definition Words (m : t) (s : S) : pset fin_word :=
+Definition FinWords (m : t) (s : S) : pset fin_word :=
   fun w => FinWord m s w.
 
 (** The language of an automata. *)
@@ -125,13 +143,13 @@ Proof.
     econstructor; eauto.
 Qed.
 
-Definition to_trace (p : fin_path) : fin_trace :=
+Definition to_fin_trace (p : fin_path) : fin_trace :=
   List.map (fun '(x, y) => y) p.
-Coercion to_trace : fin_path >-> fin_trace.
+Coercion to_fin_trace : fin_path >-> fin_trace.
 
-Definition to_word (p : fin_path) : fin_word :=
+Definition to_fin_word (p : fin_path) : fin_word :=
   List.map (fun '(x, y) => x) p.
-Coercion to_word : fin_path >-> fin_word.
+Coercion to_fin_word : fin_path >-> fin_word.
 
 Theorem FinPath_FinTrace:
   forall m x p y,
@@ -166,5 +184,62 @@ Proof.
     exists ((a, x)::p), z.
     econstructor; eauto.
 Qed.
+
+(** ** Infinite Traces, Paths and Words *)
+
+(** A path is an infinite sequence of labels and states *)
+Definition path : Type := sequence.t (A * S).
+
+(** A trace is an infinite sequence of states *)
+Definition trace : Type := sequence.t S.
+
+(** A word is an infinite sequence of labels *)
+Definition word : Type := sequence.t A.
+
+(** What it means to be a valid path *)
+Definition Path (m : t) (s0 : S) (p : path) : Prop :=
+  snd (p 0) = s0 /\
+  forall i,
+    m $ snd (p i) -[fst (p i)]-> snd (p (i + 1)).
+
+(** What it means to be an initial path *)
+Definition iPath (m : t) : pset path :=
+  fun p => exists s0, In s0 (m_initial m) /\ Path m s0 p.
+
+(** What it means to be a valid trace *)
+Definition Trace (m : t) (s0 : S) (t : trace) : Prop :=
+  t 0 = s0 /\
+  forall i,
+    m $ t i --> t (i + 1).
+
+(** What it means to be an initial trace *)
+Definition iTrace (m : t) : pset trace :=
+  fun t => exists s0, In s0 (m_initial m) /\ Trace m s0 t.
+
+Definition to_word (p : path) : word :=
+  fun i => fst (p i).
+Coercion to_word : path >-> word.
+
+Definition to_trace (p : path) : trace :=
+  fun i => snd (p i).
+Coercion to_trace : path >-> trace.
+
+(** What it means to be a valid infinite word *)
+Definition Word (m : t) (s0 : S) (w : word) : Prop :=
+  exists (p : path), Path m s0 p /\ w ≡ p.
+
+(** Language of a Büchi Automaton *)
+Definition OmegaLanguage (m : t) : pset word :=
+  fun w => exists p,
+    iPath m p /\ w ≡ p /\
+    forall i, exists j, i < j /\ In (snd (p i)) (m_final m).
+
+(** ** Reachability *)
+
+Definition Reachable (m : t) (s0 : S) : pset S :=
+  fun s => m $ s0 ->* s.
+
+Definition iReachable (m : t) : pset S :=
+  fun s => exists s0, In s0 (m_initial m) /\ m $ s0 ->* s.
 
 End Model.
