theories/lib/sequence.v
@@ -1,0 +1,46 @@
+(** * Nat-indexed infinite sequences *)
+
+Require Import Automatik.lib.operators.
+Require Import Arith List.
+Import ListNotations.
+
+Section Sequence.
+
+Definition t (A : Type) : Type :=
+  nat -> A.
+
+Definition nth {A : Type} (s : t A) (i : nat) : A :=
+  s i.
+
+Definition equ {A : Type} (s1 s2 : t A) : Prop :=
+  forall i, s1 i = s2 i.
+
+Definition shift {A : Type} (s : t A) (i : nat) : t A :=
+  fun x => s (i + x).
+
+Lemma shift_assoc:
+  forall A (s : @t A) i j,
+    equ (shift (shift s i) j) (shift s (i + j)).
+Proof.
+  intros * n.
+  unfold shift.
+  now rewrite Nat.add_assoc.
+Qed.
+
+Fixpoint range {A : Type} (s : t A) (i j : nat) {struct j} : list A :=
+  if j <? i then []
+  else if i =? j then [s i]
+  else match j with
+  | 0 => []
+  | S j' => (range s i j') ++ [s j]
+  end.
+
+Definition repeat {A : Type} (a : A) (l : list A) : t A :=
+  fun i => List.nth (i mod (List.length l)) l a.
+
+End Sequence.
+
+Instance nth_op (A : Type) : NthOp (t A) A := nth.
+Instance shift_op (A : Type) : ShiftOp (t A) A := shift.
+Instance range_op (A : Type) : RangeOp (t A) A (list A) := range.
+Instance equ_op (A : Type) : EquOp (t A) := equ.
