theories/lib/operators.v
@@ -1,0 +1,69 @@
+Declare Scope ops.
+Delimit Scope ops with ops.
+
+Class InOp (x X : Type) :=
+  in_op_ : x -> X -> Prop.
+
+Notation "x ∈ X" := (in_op_ x X) (at level 39) : ops.
+
+Class CupOp (A : Type) :=
+  cup_op_ : A -> A -> A.
+
+Notation "x ∪ y" := (cup_op_ x y) (at level 40) : ops.
+
+Class CapOp (A : Type) :=
+  cap_op_ : A -> A -> A.
+
+Notation "x ∩ y" := (cap_op_ x y) (at level 40) : ops.
+
+Class SubsetOp (A : Type) :=
+  subset_op_ : A -> A -> Prop.
+
+Notation "x ⊂ y" := (subset_op_ x y) (at level 39) : ops.
+
+Class SubseteqOp (A : Type) :=
+  subseteq_op_ : A -> A -> Prop.
+
+Notation "x ⊆ y" := (subseteq_op_ x y) (at level 39) : ops.
+
+Class StepOp (A B : Type) :=
+  step_op_ : A -> B -> B -> Prop.
+
+Notation "x $ y --> z" := (step_op_ x y z) (at level 39) : ops.
+
+Class StepsOp (A B : Type) :=
+  steps_op_ : A -> B -> B -> Prop.
+
+Notation "x $ y ->* z" := (steps_op_ x y z) (at level 39) : ops.
+
+Class LstepOp (A B C : Type) :=
+  lstep_op_ : A -> B -> C -> B -> Prop.
+
+Notation "w $ x -[ y ]-> z" := (lstep_op_ w x y z) (at level 39) : ops.
+
+Class LstepsOp (A B C : Type) :=
+  lsteps_op_ : A -> B -> C -> B -> Prop.
+
+Notation "w $ x -[ y ]->* z" := (lsteps_op_ w x y z) (at level 39) : ops.
+
+Class NthOp (A B : Type) :=
+  nth_op_ : A -> nat -> B.
+
+Notation "x ⟨ i ⟩" := (nth_op_ x i) (at level 40) : ops.
+
+Class ShiftOp (A B : Type) :=
+  shift_op_ : A -> nat -> A.
+
+Notation "x '⟨' i '+⟩'" := (shift_op_ x i) (at level 40) : ops.
+
+Class RangeOp (A B C : Type) :=
+  range_op_ : A -> nat -> nat -> C.
+
+Notation "x '⟨' i … j '⟩'" := (range_op_ x i j) (at level 40) : ops.
+
+Class EquOp (A : Type) :=
+  equ_op_ : A -> A -> Prop.
+
+Notation "x ≡ y" := (equ_op_ x y) (at level 40) : ops.
+
+Open Scope ops.
